vale/code/crypto/aes/OptPublic.fsti
@@ -3,3 +3,5 @@ module OptPublic
 open Types_s
 
 val hkeys_reqs_pub (hkeys:FStar.Seq.seq quad32) (h_LE:quad32) : Prop_s.prop0
+
+val get_hkeys_reqs (h_LE:quad32) : (s:Seq.lseq quad32 10{hkeys_reqs_pub s h_LE})
